specify iterable CBOR arrays and use them in the semantics

src/cddl/pulse/CDDL.Pulse.AST.Types.fst
@@ -1,5 +1,5 @@
 module CDDL.Pulse.AST.Types
-include CDDL.Pulse.Types
+include CDDL.Pulse.Iterator.Array
 include CDDL.Spec.AST.Base
 open Pulse.Lib.Pervasives
 open Pulse.Lib.SeqMatch
@@ -63,6 +63,8 @@ let rec impl_type_sem
   (#bound: name_env)
   (#cbor_t: Type0)
   (vmatch: perm -> cbor_t -> Cbor.cbor -> slprop)
+  (#cbor_array_iterator_t: Type0)
+  (cbor_array_iterator_match: perm -> cbor_array_iterator_t -> list Cbor.cbor -> slprop)
   (#s_env: target_type_env bound)
   (env: rel_env s_env)
   (t: target_type { target_type_bounded bound t })
@@ -74,30 +76,38 @@ let rec impl_type_sem
   | TTDef s -> env s
   | TTElem elt -> { sem_impl_type = impl_elem_type_sem cbor_t elt; sem_rel = rel_elem_type_sem vmatch elt }
   | TTOption t ->
-    let it = impl_type_sem vmatch env t in {
+    let it = impl_type_sem vmatch cbor_array_iterator_match env t in {
       sem_impl_type = option it.sem_impl_type;
       sem_rel = rel_option it.sem_rel
     }
   | TTPair t1 t2 ->
-    let it1 = impl_type_sem vmatch env t1 in
-    let it2 = impl_type_sem vmatch env t2 in {
+    let it1 = impl_type_sem vmatch cbor_array_iterator_match env t1 in
+    let it2 = impl_type_sem vmatch cbor_array_iterator_match env t2 in {
       sem_impl_type = (it1.sem_impl_type & it2.sem_impl_type);
       sem_rel = rel_pair it1.sem_rel it2.sem_rel
     }
   | TTUnion t1 t2 ->
-    let it1 = impl_type_sem vmatch env t1 in
-    let it2 = impl_type_sem vmatch env t2 in {
+    let it1 = impl_type_sem vmatch cbor_array_iterator_match env t1 in
+    let it2 = impl_type_sem vmatch cbor_array_iterator_match env t2 in {
       sem_impl_type = (it1.sem_impl_type `either` it2.sem_impl_type);
       sem_rel = rel_either it1.sem_rel it2.sem_rel
     }
   | TTArray t ->
-    let it = impl_type_sem vmatch env t in {
-      sem_impl_type = slice it.sem_impl_type; // HERE we will plug support for iterable CBOR arrays whose elements will be parsed wrt. it.sem_rel
-      sem_rel = rel_slice_of_list it.sem_rel false;
+    let it = impl_type_sem vmatch cbor_array_iterator_match env t in {
+      sem_impl_type =
+        either
+          (slice it.sem_impl_type)
+          (array_iterator_t vmatch cbor_array_iterator_t it.sem_impl_type (mk_spec it.sem_rel)) // HERE the relation on the element types is used in the implementation array type
+          ;
+      sem_rel =
+        rel_either_left
+          (rel_slice_of_list it.sem_rel false)
+          (rel_array_iterator vmatch cbor_array_iterator_match it.sem_rel)
+          ;
     }
   | TTTable t1 t2 ->
-    let it1 = impl_type_sem vmatch env t1 in
-    let it2 = impl_type_sem vmatch env t2 in {
+    let it1 = impl_type_sem vmatch cbor_array_iterator_match env t1 in
+    let it2 = impl_type_sem vmatch cbor_array_iterator_match env t2 in {
       sem_impl_type = slice (it1.sem_impl_type & it2.sem_impl_type); // HERE we will plug support for iterable CBOR maps whose elements will be parsed wrt. it1.sem_rel, it2.sem_rel
       sem_rel = rel_slice_of_table (target_type_eq s_env t1) it1.sem_rel it2.sem_rel
     }
@@ -117,6 +127,8 @@ let rec impl_type_sem_incr
   (#bound1: name_env)
   (cbor_t: Type0)
   (vmatch: perm -> cbor_t -> Cbor.cbor -> slprop)
+  (#cbor_array_iterator_t: Type0)
+  (cbor_array_iterator_match: perm -> cbor_array_iterator_t -> list Cbor.cbor -> slprop)
   (#s_env1: target_type_env bound1)
   (env1: rel_env s_env1)
   (#bound2: name_env)
@@ -127,20 +139,20 @@ let rec impl_type_sem_incr
   (requires rel_env_included env1 env2 /\
     target_type_bounded bound1 t
   )
-  (ensures impl_type_sem vmatch env1 t == coerce_eq () (impl_type_sem vmatch env2 t)) // FIXME: WHY WHY WHY do we have this coerce_eq?
+  (ensures impl_type_sem vmatch cbor_array_iterator_match env1 t == coerce_eq () (impl_type_sem vmatch cbor_array_iterator_match env2 t)) // FIXME: WHY WHY WHY do we have this coerce_eq?
   (decreases t)
   [SMTPatOr [
-    [SMTPat (rel_env_included env1 env2); SMTPat (impl_type_sem vmatch env1 t);];
-    [SMTPat (rel_env_included env1 env2); SMTPat (impl_type_sem vmatch env2 t);];
+    [SMTPat (rel_env_included env1 env2); SMTPat (impl_type_sem vmatch cbor_array_iterator_match env1 t);];
+    [SMTPat (rel_env_included env1 env2); SMTPat (impl_type_sem vmatch cbor_array_iterator_match env2 t);];
   ]]
 = match t with
   | TTOption t1
   | TTArray t1
-    -> impl_type_sem_incr cbor_t vmatch env1 env2 t1
+    -> impl_type_sem_incr cbor_t vmatch cbor_array_iterator_match env1 env2 t1
   | TTPair t1 t2
   | TTUnion t1 t2
   | TTTable t1 t2 ->
     eq_test_unique (target_type_eq s_env1 t1) (coerce_eq () (target_type_eq s_env2 t1));
-    impl_type_sem_incr cbor_t vmatch env1 env2 t1;
-    impl_type_sem_incr cbor_t vmatch env1 env2 t2
+    impl_type_sem_incr cbor_t vmatch cbor_array_iterator_match env1 env2 t1;
+    impl_type_sem_incr cbor_t vmatch cbor_array_iterator_match env1 env2 t2
   | _ -> ()
