src/cddl/pulse/CDDL.Pulse.Iterator.Array.fst
@@ -1,0 +1,27 @@
+module CDDL.Pulse.Iterator.Array
+include CDDL.Pulse.Iterator.Base
+include CDDL.Pulse.Parse.Base
+open Pulse.Lib.Pervasives
+
+module Cbor = CBOR.Spec.API.Type
+module Spec = CDDL.Spec.Base
+module SM = Pulse.Lib.SeqMatch
+
+noeq
+type array_iterator_t (#cbor: Type0) (vmatch: perm -> cbor -> Cbor.cbor -> slprop) (cbor_array_iterator_t: Type0) (impl_elt: Type0) (spec: Ghost.erased (src_elt: Type0 & rel impl_elt src_elt)) : Type0 = {
+  contents: cbor_array_iterator_t;
+  pm: perm;
+  ty: Ghost.erased Spec.typ;
+  ser: Ghost.erased (dfst spec -> bool);
+  ps: Ghost.erased (Spec.parser_spec ty (dfst spec) ser);
+  impl_parse: impl_zero_copy_parse vmatch ps (dsnd spec);
+}
+
+let rel_array_iterator
+  (#cbor: Type0) (vmatch: perm -> cbor -> Cbor.cbor -> slprop) (#cbor_array_iterator_t: Type0) (cbor_array_iterator_match: perm -> cbor_array_iterator_t -> list Cbor.cbor -> slprop) (#impl_elt: Type0) (#src_elt: Type0) (r: rel impl_elt src_elt) :
+    rel (array_iterator_t vmatch cbor_array_iterator_t impl_elt (mk_spec r)) (list src_elt)
+= mk_rel (fun i s -> exists* l . cbor_array_iterator_match i.pm i.contents l **
+    pure (
+      List.Tot.map (apply_parser i.ps) l == List.Tot.map Some s
+    )
+  )
